wip: enqueue

lawyer/nonblocking/examples/queue/other_methods.v
@@ -8,7 +8,11 @@ From lawyer.obligations Require Import obligations_model obligations_resources o
 From lawyer Require Import sub_action_em program_logic.
 From iris.algebra Require Import auth gmap gset excl excl_auth csum mono_nat.
 From iris.base_logic.lib Require Import invariants.
-From lawyer.nonblocking.examples.queue Require Import simple_queue_utils simple_queue dequeue.
+From lawyer.nonblocking.examples.queue Require Import simple_queue_utils simple_queue dequeue read_head.
+From heap_lang Require Import heap_lang_defs lang notation.
+
+
+Close Scope Z.
 
 
 Section OtherMethods.
@@ -36,6 +40,180 @@ Section OtherMethods.
 
   Let hGS: heap1GS Σ := iem_phys _ EM.
   Existing Instance hGS.
+
+  Definition set_val: val := λ: "nd" "v", ("nd" +ₗ #0) <- "v".
+  Definition set_next: val := λ: "nd" "nxt", ("nd" +ₗ #1) <- "nxt".
+
+  Definition set_node: val := 
+      λ: "nd" "v" "nxt",
+        set_val "nd" "v" ;;
+        set_next "nd" "nxt"
+  .
+
+  Definition mk_dummy_node: val :=
+    λ: <>,
+      (** dummy node has concrete field values, so we have to set them *)
+      let: "nd" := AllocN (Val $ LitV $ LitInt 2) #0 in
+      set_next "nd" #(Loc 0) ;;
+      "nd"
+  .
+
+  Definition enqueue '(SQ H T BR FL OHV as sq): val :=
+    λ: "v",
+      let: "nd" := mk_dummy_node #() in
+      let: "cl" := !#T in
+      set_node "cl" "v" "nd" ;;
+      #T <- "nd"
+  .
+
+  (** TODO: move, remove duplicates *)
+  Definition mk_node_fuel := 20.
+
+  Lemma set_node_spec (τ: locale heap_lang) (π: Phase) (q: Qp) (pt: loc) nd (v: val) (nxt: loc):
+    {{{ th_phase_frag τ π q ∗ cp_mul π d mk_node_fuel ∗ hn_interp (pt, nd) }}}
+       set_node #pt v #nxt @τ
+    {{{ RET #(); th_phase_frag τ π q ∗ hn_interp (pt, (v, nxt)) }}}.
+  Proof using.
+    destruct nd. iIntros (Φ) "(PH & CPS & (V & NXT)) POST".
+    rewrite /set_node. pure_steps.
+    rewrite /set_val. pure_steps.
+
+    wp_bind (_ +ₗ _)%E.
+    iApply sswp_MU_wp; [done| ].
+    iApply sswp_pure_step.
+    { rewrite /bin_op_eval. erewrite decide_False; [| done]. reflexivity. }
+    MU_by_burn_cp. iApply wp_value.
+
+    iApply sswp_MU_wp; [done| ].
+    rewrite loc_add_0. iApply (wp_store with "V").
+    iIntros "!> V".
+    MU_by_burn_cp. iApply wp_value.
+
+    wp_bind (Rec _ _ _)%E. pure_steps.
+    rewrite /set_next. pure_steps.
+
+    wp_bind (_ +ₗ _)%E.
+    iApply sswp_MU_wp; [done| ].
+    iApply sswp_pure_step.
+    { rewrite /bin_op_eval. erewrite decide_False; [| done]. reflexivity. }
+    MU_by_burn_cp. iApply wp_value. 
+ 
+    iApply sswp_MU_wp; [done| ].
+    iApply (wp_store with "NXT").
+    iIntros "!> NXT".
+    MU_by_burn_cp. iApply wp_value.
+
+    iApply "POST". iFrame.
+  Qed.    
+
+  Lemma mk_dummy_node_spec (τ: locale heap_lang) (π: Phase) (q: Qp):
+    {{{ th_phase_frag τ π q ∗ cp_mul π d mk_node_fuel }}}
+       mk_dummy_node #() @τ
+    {{{ (pt: loc), RET #pt; th_phase_frag τ π q ∗ hn_interp (pt, dummy_node) }}}.
+  Proof using.
+    iIntros (Φ) "(PH & CPS) POST". rewrite /mk_dummy_node.
+    pure_steps.
+
+    wp_bind (AllocN _ _)%E.
+    iApply sswp_MU_wp; [done| ].
+    iApply wp_allocN_seq.
+    { lia. }
+    iIntros "!>" (pt) "LS". simpl.
+    iDestruct "LS" as "((V & _) & (NXT & _) & _)". 
+    MU_by_burn_cp. iApply wp_value.
+
+    wp_bind (Rec _ _ _)%E. pure_steps.
+    rewrite /set_next. pure_steps.
+
+    wp_bind (_ +ₗ _)%E.
+    iApply sswp_MU_wp; [done| ].
+    iApply sswp_pure_step.
+    { rewrite /bin_op_eval. erewrite decide_False; [| done]. reflexivity. }
+    MU_by_burn_cp. iApply wp_value. 
+ 
+    iApply sswp_MU_wp; [done| ].
+    iApply (wp_store with "[$]").
+    iIntros "!> NXT".
+    MU_by_burn_cp. iApply wp_value.
+
+    wp_bind (Rec _ _ _)%E. pure_steps.
+    rewrite loc_add_0. 
+    iApply "POST". iFrame.
+  Qed.
+
+  Definition enqueue_fuel := 100.
+
+  Lemma start_enqueue l (τ: locale heap_lang) (π: Phase) (q: Qp):
+    {{{ queue_inv l ∗ read_head_token ∗ 
+        th_phase_frag τ π q ∗ cp_mul π d 1 }}}
+       !#(Tail q_sq) @ τ
+    {{{ (pt: loc), RET #pt; th_phase_frag τ π q ∗ rop_token ∗ 
+          ∃ t br rop, read_head_resources t br pt rop }}}.
+  Proof using.
+    simpl. iIntros (Φ) "([#QAT #INV] & TOK & PH & CPS) POST".
+    iInv "INV" as "(%hq & %h & %t & %br & %fl & %rop & %od & %hist & inv)" "CLOS".
+    iEval (rewrite /queue_inv_inner) in "inv".
+    iDestruct "inv" as ">(HQ & AUTHS & %ORDER0 & QI & DANGLE & OHV & RHI & RH & DQ)".
+    
+    iApply sswp_MU_wp; [done| ].
+    iDestruct (access_queue_ends with "[$] [$]") as "(%ph & %pt & HEAD & TAIL & #HT & CLOS')".    
+    iApply (wp_load with "TAIL"). iIntros "!> TAIL".
+    iDestruct "RH" as "[(%pt_ & RH & RTOK) | TOK']".
+    2: { by iDestruct (read_head_token_excl with "[$] [$]") as "?". }
+    iDestruct (read_head_res_Tail_agree with "RH [$]") as %EQ.
+    inversion EQ. subst pt_. clear EQ. 
+      
+    iDestruct ("CLOS'" with "[$] [$]") as "(HQ & QI)".
+    MU_by_burn_cp. iApply wp_value.
+
+    iApply "POST". iFrame.
+
+    iMod ("CLOS" with "[-]") as "_"; [| done].
+    by iFrame.
+  Qed.    
+
+  Lemma enqueue_spec l (τ: locale heap_lang) (π: Phase) (q: Qp) (v: val):
+    {{{ queue_inv l ∗ read_head_token ∗ 
+        th_phase_frag τ π q ∗ cp_mul π d enqueue_fuel }}}
+       enqueue q_sq l v @ τ
+    {{{ (v: val), RET v; th_phase_frag τ π q ∗ read_head_token }}}.
+  Proof using.
+    simpl. iIntros (Φ) "([#QAT #INV] & TOK & PH & CPS) POST".
+    rewrite /enqueue. destruct q_sq eqn:Q_SQ.
+    pure_steps.
+
+    split_cps "CPS" mk_node_fuel; [cbv; lia| ]. 
+    iApply (mk_dummy_node_spec with "[$CPS' $PH]").
+    iIntros "!>" (pn) "(PH & NI)".
+
+    wp_bind (Rec _ _ _)%E. pure_steps.
+
+    wp_bind (! _)%E.
+    split_cps "CPS" 1.
+    replace Tail with (simple_queue.Tail q_sq) by (by rewrite Q_SQ).
+    iApply (start_enqueue with "[$QAT $INV $CPS' $PH $TOK]").
+    iIntros "!> %pt (PH & RTOK & (%t & %br & %rop & RH))".
+
+    wp_bind (Rec _ _ _)%E. do 3 pure_step_cases.
+
+    wp_bind (set_node _ _ _)%E.
+    split_cps "CPS" mk_node_fuel; [cbv; lia| ]. 
+    iApply (set_node_spec with "[$CPS' $PH NI]").
+    { 
+
+    
+    wp_bind (Rec _ _ _)%E. pure_steps.
+    wp_bind (_ = _)%E.
+    iApply sswp_MU_wp; [done| ].
+    iApply sswp_pure_step.
+    { set_solver. }
+    MU_by_burn_cp. iApply wp_value.
+
+
+
+    
+
+      
 
   Definition read_head_dequeuer_fuel := 100.
 
